Lp2lc/Active.lean
@@ -3,3 +3,4 @@ import «Lp2lc».Active.FsubL_alt
 import «Lp2lc».Active.Dsub
 import «Lp2lc».Active.Dsubsup
 import «Lp2lc».Active.Ddia
+import «Lp2lc».Active.Dot
