Lp2lc/Active/FsubL_alt.lean
@@ -1,3 +1,0 @@
-import «Lp2lc».Active.FsubL_alt.Def
-import «Lp2lc».Active.FsubL_alt.Auxiliary
-import «Lp2lc».Active.FsubL_alt.Proof
